x86/SymbtableDecode.v
@@ -1,0 +1,515 @@
+(* *******************  *)
+(* Author: Pierre Wilke *)
+(* Date:   Dec 04, 2019 *)
+(* *******************  *)
+
+(** * Decoding of the symbol table from a section *)
+
+Require Import Coqlib Integers AST Maps.
+Require Import Asm.
+Require Import Errors.
+Require Import RelocProgram Encode.
+Require Import SeqTable Memdata.
+Require Import Hex Bits.
+Import Hex Bits.
+Import ListNotations.
+Require Import SymbtableEncode.
+
+Set Implicit Arguments.
+
+Local Open Scope error_monad_scope.
+Local Open Scope hex_scope.
+Local Open Scope bits_scope.
+
+Definition decode_symbtype (z: Z) : res symbtype :=
+  match z with
+  | 0 => OK symb_notype
+  | 1 => OK symb_data
+  | 2 => OK symb_func
+  | _ => Error (msg "decode_symbtype: Unexpected value for symbtype")
+  end.
+
+Lemma decode_encode_symbtype st:
+  decode_symbtype (encode_symbtype st) = OK st.
+Proof.
+  destruct st; reflexivity.
+Qed.
+
+
+Definition decode_bindtype (z: Z) : res bindtype :=
+  match z with
+  | 0 => OK bind_local
+  | 1 => OK bind_global
+  | _ => Error (msg "decode_bindtype: Unexpected value for bindtype")
+  end.
+
+Lemma decode_encode_bindtype bt:
+  decode_bindtype (encode_symbbind bt) = OK bt.
+Proof.
+  destruct bt; reflexivity.
+Qed.
+
+
+
+Definition decode_glob_symb_info (z: Z) :=
+  let st := z mod 16 in
+  let bt := z / 16 in
+  do st <- decode_symbtype st;
+    do bt <- decode_bindtype bt;
+    OK (st, bt).
+
+Lemma decode_encode_glob_symb_info st bt :
+  decode_glob_symb_info (encode_glob_symb_info bt st) = OK (st, bt).
+Proof.
+  unfold decode_glob_symb_info, encode_glob_symb_info.
+  change (2 ^ 4) with 16.
+  rewrite Z.add_comm, Z_mod_plus_full, <- Z.add_comm.
+  rewrite Z_div_plus_full_l by omega.
+  rewrite Z.div_small, Z.mod_small, Z.add_0_r.
+  rewrite decode_encode_symbtype, decode_encode_bindtype. reflexivity.
+  destruct st; simpl; omega.
+  destruct st; simpl; omega.
+Qed.
+
+Definition decode_secindex (lb: list byte) : res secindex :=
+  let i := decode_int lb in
+  if zeq i (HZ["FFF2"])
+  then OK secindex_comm
+  else if zeq i 0
+       then OK secindex_undef
+       else
+         OK (secindex_normal (Z.to_N i)).
+
+Definition valid_secindex (i: secindex) :=
+  match i with
+  | secindex_normal idx => 0 < Z.of_N idx < HZ["FFF2"]
+  | secindex_comm => True
+  | secindex_undef => True
+  end.
+
+Lemma decode_encode_secindex i (V: valid_secindex i):
+  decode_secindex (encode_secindex i) = OK i.
+Proof.
+  unfold decode_secindex, encode_secindex.
+  rewrite decode_encode_int.
+  destruct i; try reflexivity.
+  simpl in V.
+  rewrite Z.mod_small. rewrite pred_dec_false. rewrite pred_dec_false.
+  rewrite N2Z.id. auto. omega. simpl. omega.
+  change (two_p (Z.of_nat 2 * 8)) with 65536. omega.
+Qed.
+Record valid_symbentry strtab (e: symbentry) : Prop :=
+  {
+    valid_symbentry_size: 0 <= symbentry_size e < two_p 32;
+    valid_symbentry_value: 0 <= symbentry_value e < two_p 32;
+    valid_symbentry_id: forall id, symbentry_id e = Some id ->
+                                   exists si, strtab ! id  = Some si /\ 0 <= si < two_p 32;
+    valid_symbentry_secindex: valid_secindex (symbentry_secindex e);
+  }.
+
+Record valid_strtable (strtab: strtable) : Prop :=
+  {
+    nodupstr: forall i j x y,
+      strtab ! i = Some x -> strtab ! j = Some y -> i <> j -> x <> y;
+    strtab_no_0:
+      forall i : positive, strtab ! i = Some 0 -> False;
+  }.
+
+
+Section WITH_STRTAB.
+
+Variable (strtab: strtable).
+
+Hypothesis valid_strtab: valid_strtable strtab.
+
+Fixpoint take_drop {A} n (l: list A) : res (list A * list A) :=
+  match n, l with
+  | O, l => OK ([], l)
+  | S n, a::r =>
+    do (a1,b1) <- take_drop n r ;
+    OK (a::a1, b1)
+  | S n, [] => Error (msg "take_drop: list too short")
+  end.
+
+Definition strtab_inv si : option ident :=
+  PTree.fold (fun acc id val =>
+                match acc with
+                | Some _ => acc
+                | None =>
+                  if zeq val si then Some id else acc
+                end
+             ) strtab None.
+
+Definition decode_symbentry (lb: list byte) : res symbentry :=
+  do (st_name_bytes, lb) <- take_drop 4 lb;
+    do (st_value_bytes, lb) <- take_drop 4 lb;
+    do (st_size_bytes, lb) <- take_drop 4 lb;
+    do (st_info_bytes, lb) <- take_drop 1 lb;
+    do (st_other_bytes, lb) <- take_drop 1 lb;
+    do (st_shndx_bytes, lb) <- take_drop 2 lb;
+
+    let name_index := decode_int32 st_name_bytes in
+    let svalue := decode_int32 st_value_bytes in
+    let ssize := decode_int32 st_size_bytes in
+    do (st, bt) <- decode_glob_symb_info (decode_int st_info_bytes);
+      do secindex <- decode_secindex st_shndx_bytes;
+      let sid := strtab_inv name_index in
+      OK (
+          {|
+            symbentry_id := sid;
+            symbentry_bind := bt;
+            symbentry_type := st;
+            symbentry_value := svalue;
+            symbentry_secindex := secindex;
+            symbentry_size := ssize
+          |}
+        ).
+
+Lemma take_drop_encode_int sz x l:
+  take_drop sz (encode_int sz x ++ l) = OK (encode_int sz x, l).
+Proof.
+  generalize (encode_int_length sz x).
+  generalize (encode_int sz x).
+  induction sz; simpl; intros; eauto.
+  - destruct l0; simpl in *; try congruence.
+  - destruct l0; simpl in *; try congruence.
+    rewrite IHsz. simpl. auto. congruence.
+Qed.
+
+Lemma take_drop_cons {A} x (l: list A):
+  take_drop 1 (x :: l) = OK ([x], l).
+Proof.
+  reflexivity.
+Qed.
+
+
+Lemma take_drop_length {A} sz (l: list A):
+  length l = sz ->
+  take_drop sz l = OK (l, []).
+Proof.
+  revert l.
+  induction sz; simpl; intros; eauto.
+  - destruct l; simpl in *; try congruence.
+  - destruct l; simpl in *; try congruence.
+    rewrite IHsz. simpl. auto. congruence.
+Qed.
+
+
+Lemma take_drop_length_app {A} sz (l1 l2: list A):
+  length l1 = sz ->
+  take_drop sz (l1 ++ l2) = OK (l1, l2).
+Proof.
+  revert l1 l2.
+  induction sz; simpl; intros; eauto.
+  - destruct l1; simpl in *; try congruence.
+  - destruct l1; simpl in *; try congruence.
+    rewrite IHsz. simpl. auto. congruence.
+Qed.
+
+
+Lemma take_drop_length_2 :
+  forall {A} z (l: list A) l1 l2,
+    (z > 0)%nat ->
+    take_drop z l = OK (l1, l2) ->
+    (length l2 < length l)%nat.
+Proof.
+  induction z; simpl; intros; eauto. omega.
+  destr_in H10. monadInv H10.
+  destruct z.  simpl in *. inv EQ.  omega.
+  apply IHz in EQ. simpl. omega. omega.
+Qed.
+
+Lemma fold_left_strtab_inv_stable:
+  forall x l i,
+  fold_left
+    (fun (a : option positive) (p : positive * Z) =>
+     match a with
+     | Some _ => a
+     | None => if zeq (snd p) x then Some (fst p) else a
+     end) l (Some i) = Some i.
+Proof.
+  induction l; simpl; intros; eauto.
+Qed.
+
+Lemma strtab_inv_ok
+  : forall i x,
+    strtab ! i = Some x ->
+    strtab_inv x = Some i.
+Proof.
+  unfold strtab_inv.
+  intros i x EQ.
+  apply PTree.elements_correct in EQ.
+  rewrite PTree.fold_spec.
+  revert EQ.
+  assert (list_norepet (map snd (PTree.elements strtab))).
+  {
+
+    generalize (PTree.elements_complete strtab).
+    generalize (PTree.elements_keys_norepet strtab).
+    generalize (PTree.elements strtab).
+    induction l; simpl; intros; eauto. constructor.
+    constructor.
+    - intro IN. rewrite in_map_iff in IN. destruct IN as ((xx & y) & EQ & IN).
+      simpl in EQ. subst. inv H.
+      destruct a; simpl in *.
+      clear IHl.
+      generalize (H10 _ _ (or_introl eq_refl)).
+      generalize (H10 _ _ (or_intror IN)). intros A B.
+      apply (nodupstr valid_strtab A B); auto. intro; subst.
+      apply H13. eapply in_map_iff. eexists; split; eauto. reflexivity.
+    - apply IHl. inv H; auto. intros; eauto.
+  } revert H.
+  generalize (PTree.elements strtab).
+  induction l; simpl; intros. easy.
+  destruct EQ as [EQ|IN].
+  - subst. simpl. rewrite zeq_true.
+    apply fold_left_strtab_inv_stable.
+  - inv H. rewrite zeq_false. auto. intro; subst. apply H12.
+    apply in_map_iff.
+    eexists; split. 2: apply IN. reflexivity.
+Qed.
+
+Lemma strtab_inv_none
+  : forall x,
+    (forall i, strtab ! i = Some x -> False) ->
+    strtab_inv x = None.
+Proof.
+  unfold strtab_inv.
+  intros x NEQ.
+  assert (~ In x (map snd (PTree.elements strtab))).
+  {
+    intro IN.
+    rewrite in_map_iff in IN. destruct IN as (x0 & EQ & IN).
+    destruct x0; simpl in *; subst.
+    apply PTree.elements_complete in IN. eapply NEQ. eauto.
+  } clear NEQ.
+  rewrite PTree.fold_spec.
+  revert H.
+  assert (list_norepet (map snd (PTree.elements strtab))).
+  {
+
+    generalize (PTree.elements_complete strtab).
+    generalize (PTree.elements_keys_norepet strtab).
+    generalize (PTree.elements strtab).
+    induction l; simpl; intros; eauto. constructor.
+    constructor.
+    - intro IN. rewrite in_map_iff in IN. destruct IN as ((xx & y) & EQ & IN).
+      simpl in EQ. subst. inv H.
+      destruct a; simpl in *.
+      clear IHl.
+      generalize (H10 _ _ (or_introl eq_refl)).
+      generalize (H10 _ _ (or_intror IN)). intros A B.
+      apply (nodupstr valid_strtab A B); auto. intro; subst.
+      apply H13. eapply in_map_iff. eexists; split; eauto. reflexivity.
+    - apply IHl. inv H; auto. intros; eauto.
+  } revert H.
+  generalize (PTree.elements strtab).
+  induction l; simpl; intros. auto.
+  rewrite zeq_false. 2: intuition congruence.
+  apply IHl. inv H; auto. intuition.
+Qed.
+
+
+
+
+
+Lemma encode_symbbind_range:
+  forall sb,
+    0 <= encode_symbbind sb < two_p 4.
+Proof.
+  unfold encode_symbbind.
+  intros; destr; vm_compute; intuition congruence.
+Qed.
+
+Lemma encode_symbtype_range:
+  forall sb,
+    0 <= encode_symbtype sb < two_p 4.
+Proof.
+  unfold encode_symbtype.
+  intros; destr; vm_compute; intuition congruence.
+Qed.
+Require Import Psatz.
+Lemma encode_glob_symb_info_range:
+  forall sb st,
+    0 <= encode_glob_symb_info sb st < two_p 8.
+Proof.
+  unfold encode_glob_symb_info.
+  intros.
+  generalize (encode_symbbind_range sb) (encode_symbtype_range st).
+  intros. split. lia.
+  change (two_p 8) with (2 ^ 8).
+  apply Z.add_nocarry_lt_pow2.
+  change (2 ^ 4) with (two_p 4).
+  rewrite <- Byte.Zshiftl_mul_two_p.
+  apply Byte.equal_same_bits.
+  intros. rewrite Byte.Ztestbit_0.
+  rewrite Z.land_spec.
+  destruct (zlt i 4).
+  rewrite Z.shiftl_spec_low. reflexivity. auto.
+  apply andb_false_intro2.
+  apply Byte.Ztestbit_above with (n:=4%nat).
+  change (two_power_nat 4) with (two_p 4); auto. simpl; auto. omega.
+  change (2 ^ 8) with (two_p 4 * 2 ^ 4).
+  apply Zmult_lt_compat_r. lia. apply H.
+  cut (two_p 4 < 2 ^ 8). lia. vm_compute; intuition congruence.
+Qed.
+
+
+Lemma decode_encode_symbentry e (V: valid_symbentry strtab e) lb:
+  encode_symbentry strtab e = OK lb ->
+  decode_symbentry lb = OK e.
+Proof.
+  unfold encode_symbentry, decode_symbentry.
+  intros A. monadInv A.
+  Opaque take_drop.
+  rewrite take_drop_encode_int. simpl.
+  rewrite take_drop_encode_int. simpl.
+  rewrite take_drop_encode_int. simpl.
+  rewrite take_drop_cons. simpl.
+  rewrite take_drop_cons. simpl.
+  rewrite take_drop_length. simpl.
+  assert (forall x, [Byte.repr x] = encode_int 1 x).
+  {
+    clear.
+    unfold encode_int. simpl.
+    unfold rev_if_be. intros; destr.
+  }
+  rewrite H.
+  rewrite decode_encode_int.
+  rewrite Z.mod_small.
+  rewrite decode_encode_glob_symb_info. simpl.
+  rewrite decode_encode_secindex. simpl.
+  rewrite decode_encode_int. rewrite Z.mod_small.
+  rewrite decode_encode_int. rewrite Z.mod_small.
+  rewrite decode_encode_int. rewrite Z.mod_small.
+  f_equal. destruct e; f_equal.
+  simpl in *. destr_in EQ. destr_in EQ. inv EQ.
+  eapply strtab_inv_ok. auto.
+  apply strtab_inv_none. inv EQ. apply strtab_no_0. auto.
+  eapply valid_symbentry_size; eauto.
+  eapply valid_symbentry_value; eauto.
+  destr_in EQ.
+  edestruct valid_symbentry_id as (id & EQid & IN); eauto.
+  rewrite EQid in EQ. inv EQ. auto.
+  inv EQ.
+  split. omega. apply Z.gt_lt. apply two_p_gt_ZERO. omega.
+  eapply valid_symbentry_secindex. eauto.
+  apply encode_glob_symb_info_range.
+  unfold encode_secindex.
+  rewrite encode_int_length.
+  auto.
+Qed.
+
+Program Fixpoint decode_symbentries l {measure (length l)} : res (list symbentry) :=
+  match l with
+    [] => OK []
+  | _ => match take_drop 16 l with
+         | OK (e, r) =>
+           do e <- decode_symbentry e;
+             do r <- decode_symbentries r;
+             OK (e::r)
+         | Error m => Error m
+         end
+  end.
+Next Obligation.
+  eapply take_drop_length_2. 2: eauto. omega.
+Defined.
+
+Lemma decode_symbentries_eq l:
+  decode_symbentries l =
+  match l with
+    [] => OK []
+  | _ => match take_drop 16 l with
+         | OK (e, r) =>
+           do e <- decode_symbentry e;
+             do r <- decode_symbentries r;
+             OK (e::r)
+         | Error m => Error m
+         end
+  end.
+Proof.
+Admitted.
+
+Lemma encode_secindex_length i:
+  length (encode_secindex i) = 2%nat.
+Proof.
+  unfold encode_secindex. rewrite encode_int_length. auto.
+Qed.
+
+Lemma encode_symbentry_length e l:
+  encode_symbentry strtab e = OK l ->
+  length l = 16%nat.
+Proof.
+  unfold encode_symbentry. intro A. monadInv A.
+  rewrite ! app_length.
+  unfold encode_int32.
+  rewrite ! encode_int_length.
+  simpl.
+  rewrite encode_secindex_length.
+  auto.
+Qed.
+
+Lemma decode_encode_symtable t (V: Forall (valid_symbentry strtab) t) lb:
+  encode_symbtable strtab t = OK lb ->
+  decode_symbentries lb = OK t.
+Proof.
+  unfold encode_symbtable.
+  revert lb.
+  induction t; simpl; intros; eauto.
+  - inv H; auto. 
+  - unfold acc_bytes in H. monadInv H.
+    rewrite decode_symbentries_eq.
+    generalize (encode_symbentry_length _ EQ1). intro L.
+    rewrite take_drop_length_app; auto.
+    erewrite decode_encode_symbentry. 3: eauto. 2: inv V; auto.
+    destr. destruct x0; simpl in *; congruence.
+    simpl.
+    rewrite IHt. simpl. auto.
+    inv V; auto. auto.
+Qed.
+
+Definition decode_symtable_section (s: section) : res symbtable :=
+  match s with
+  | sec_bytes bytes => decode_symbentries bytes
+  | _ => Error (msg "decode_symtable_section: should be a bytes section")
+  end.
+
+Lemma decode_create_symtable_section t (V: Forall (valid_symbentry strtab) t) s :
+  create_symbtable_section strtab t = OK s ->
+  decode_symtable_section s = OK t.
+Proof.
+  intros A. unfold create_symbtable_section in A. monadInv A.
+  simpl. eapply decode_encode_symtable; eauto.
+Qed.
+
+End WITH_STRTAB.
+
+
+Definition correct_encoding_symtable_program p : Prop :=
+  match nth_error (prog_sectable p) 4 with
+  | None => False
+  | Some s =>
+    match decode_symtable_section (prog_strtable p) s with
+    | OK s => prog_symbtable p = s
+    | _ => False
+    end
+  end.
+
+Lemma transf_program_correct p
+      (V: valid_strtable (prog_strtable p))
+      (VE: Forall (valid_symbentry (prog_strtable p)) (prog_symbtable p))
+      p' (TF: transf_program p = OK p'):
+  correct_encoding_symtable_program p'.
+Proof.
+  unfold transf_program in TF. monadInv TF.
+  destr_in EQ0. simpl in *. inv EQ0.
+  red. simpl.
+  destruct (prog_sectable p); simpl in *; try congruence.
+  destruct s0; simpl in *; try congruence.
+  destruct s1; simpl in *; try congruence.
+  destruct s2; simpl in *; try congruence.
+  destruct s3; simpl in *; try congruence.
+  erewrite decode_create_symtable_section; eauto.
+  apply beq_nat_true in Heqb.
+  rewrite app_length in Heqb. simpl in Heqb. omega.
+Qed.
